Put all types in Interpreter.Types

Interpreter/Types/Identifier.lean
@@ -1,58 +1,7 @@
-import AssertCmd
+import Interpreter.Types.Name
 
 
-section Name
-
-
-def Name.isHead (c : Char) := c.isAlpha || c == '_'
-def Name.isTail (c : Char) := c.isAlphanum || c ∈ "_'+-".toList
-abbrev Name.Head := Subtype (isHead .)
-abbrev Name.Tail := Subtype (isTail .)
-
-
-structure Name where
-  head : Name.Head
-  tail : List Name.Tail
-  deriving DecidableEq, Hashable
-
-
-def Name.toList (name : Name) : List Char :=
-  name.head.val :: name.tail.map (·.val)
-
-
-def Name.toString (name : Name) : String := name.toList.asString
-
-
-instance : ToString Name where toString name := name.toString
-
-
-instance : Repr Name where
-  reprPrec name n := toString name |> (reprPrec . n)
-
-
-def Name.of (str : List Char) : Option Name :=
-  match str with
-  | [] => none
-  | head :: tail =>
-    if h_head : isHead head then
-      if h_tail : ∀ c ∈ tail, isTail c then
-        let tail := tail.attachWith _ h_tail
-        some <| Name.mk (Subtype.mk _ h_head) tail
-      else none
-    else none
-
-
-#assert (Name.of "yogev".toList |>.isSome) == true
-
-
-instance : Inhabited Name := by
-  let x := Name.of "a".toList
-  have h : x.isSome := by decide
-  constructor
-  exact x.get h
-
-
-end Name
+namespace Interpreter.Types
 
 
 inductive Ident
