Interpreter.lean
@@ -1,10 +1,7 @@
--- This module serves as the root of the `InterpreterTest` library.
--- Import modules here that should be built as part of the library.
-import Interpreter.Basic
+import Interpreter.Types
 import Interpreter.Lex
 import Interpreter.Parse
 import Interpreter.Check
--- TODO: implement an evaluation module
 import Interpreter.Eval
 
 namespace Interpreter
