Interpreter/Check.lean
@@ -1,9 +1,13 @@
 import Interpreter.Types.Ast
-import Interpreter.Basic -- Expr
+import Interpreter.Types
+open Interpreter.Types (Expr Ty VarTypes Ast Name)
+
+
+abbrev SomeExpr := (ty : Ty) × (vt : VarTypes) × Expr ty vt
 
 -- TODO: Rename to Check.Error (preferably by using a namespace decl)
 inductive Error
-| NameIsNotDefined (name : String) (vars : VarTypes) : Error
+| NameIsNotDefined (name : Name) (vars : VarTypes) : Error
 | Many : List Error -> Error
 | TypesCannotBeAdded : SomeExpr -> SomeExpr -> Error
 deriving Inhabited, Repr
@@ -22,25 +26,24 @@ def Except.elim2 {α β e ε}
 def checkWithEnv env : Ast -> Except Error ((ty : Ty) × Expr ty env)
   | Ast.val int => ok ⟨Ty.int, Expr.val int⟩
   | Ast.var (.name name) => 
-    if h : name.toString ∈ env
-    then ok ⟨env[name.toString], Expr.var name.toString⟩
-    else error (Error.NameIsNotDefined name.toString env)
-  | Ast.add e1 e2 =>
-    Except.elim2
-      (fun
-        | ⟨Ty.int, e1⟩, ⟨Ty.int, e2⟩ => ok ⟨Ty.int, Expr.add e1 e2⟩
-        | ⟨_, e1⟩, ⟨_, e2⟩ =>
-          error (Error.TypesCannotBeAdded ⟨_, _, e1⟩ ⟨_, _, e2⟩))
-      id
-      (fun e1 e2 => Error.Many [e1, e2])
-      (checkWithEnv env e1)
-      (checkWithEnv env e2)
-    |>.bind id
-  | Ast.letIn (.name name) var_expr ret_expr => do
-    let var := name.toString
+    if h : name ∈ env
+    then ok ⟨env[name], Expr.var ⟨name, h⟩⟩
+    else error (Error.NameIsNotDefined name env)
+  -- | Ast.add e1 e2 =>
+  --   Except.elim2
+  --     (fun
+  --       | ⟨Ty.int, e1⟩, ⟨Ty.int, e2⟩ => ok ⟨Ty.int, Expr.add e1 e2⟩
+  --       | ⟨_, e1⟩, ⟨_, e2⟩ =>
+  --         error (Error.TypesCannotBeAdded ⟨_, _, e1⟩ ⟨_, _, e2⟩))
+  --     id
+  --     (fun e1 e2 => Error.Many [e1, e2])
+  --     (checkWithEnv env e1)
+  --     (checkWithEnv env e2)
+  --   |>.bind id
+  | Ast.letIn (.name var) var_expr ret_expr => do
     let ⟨var_type, var_expr'⟩ <- checkWithEnv env var_expr
     let env' := env.insert var var_type
     let ⟨ty, ret_expr'⟩ <- checkWithEnv env' ret_expr
-    pure ⟨ty, Expr.let_ var var_expr' ret_expr'⟩
+    pure ⟨ty, Expr.letIn var var_expr' ret_expr'⟩
 
 def check : Ast -> Except Error ((ty : Ty) × Expr ty ∅) := checkWithEnv ∅
