Interpreter/Eval.lean
@@ -1,15 +1,27 @@
-import Interpreter.Basic
+import Interpreter.Types
 
 
 namespace Interpreter.Eval
 
 
-partial def eval {ty vars} (values : VarValues vars) (expr : Expr ty vars) : Val ty :=
+open Interpreter.Types (
+  VarValues
+  VarTypes
+  Expr
+  Val
+)
+
+
+partial def eval {ty vars} (values : VarValues vars) (expr : Expr ty vars)
+: Val ty :=
   match expr with
   | Expr.val v => v
-  | Expr.var v => values.get v
-  | Expr.add lhs rhs => eval values lhs + eval values rhs
-  | Expr.let_ var rhs ret =>
+  | Expr.var v =>
+    -- values[v.val].snd
+    have : values[v.val].fst = vars[v.val] := VarValues.fst_getElem
+    this ▸ values[v.val].snd
+  -- | Expr.add lhs rhs => eval values lhs + eval values rhs
+  | Expr.letIn var rhs ret =>
     let varValue := eval values rhs
     let values' := values.insert var varValue
     eval values' ret
