Interpreter/Types/Expr.lean
@@ -1,0 +1,26 @@
+import Interpreter.Types.Ty
+import Interpreter.Types.Vars
+
+
+namespace Interpreter.Types
+
+
+inductive Expr : Ty -> VarTypes -> Type where
+  | val {ty vt} : Val ty -> Expr ty vt
+  | var {vt} : (var : Key vt) -> Expr vt[var.val] vt
+  | letIn {ty var_ty vt}
+  : (var : Name) -> Expr var_ty vt -> Expr ty (vt.insert var var_ty) -> Expr ty vt
+  deriving Repr
+  -- deriving Repr, BEq
+  -- deriving Repr, DecidableEq
+
+
+instance {ty vt} : Inhabited (Expr ty vt) where default := .val default
+/-
+instance {ty vt} : BEq (Expr ty vt) where
+  beq
+    | .val a, .val b => a == b
+    | .var a, .var b => a == b
+    | .letIn a b c, .letIn d e f => a == d && b == e && c == f
+    | _, _ => false
+-/
