Interpreter/Types/Name.lean
@@ -1,0 +1,50 @@
+import AssertCmd
+
+
+namespace Interpreter.Types
+
+
+def Name.isHead (c : Char) := c.isAlpha || c == '_'
+def Name.isTail (c : Char) := c.isAlphanum || c ∈ "_'+-".toList
+abbrev Name.Head := Subtype (isHead .)
+abbrev Name.Tail := Subtype (isTail .)
+
+
+structure Name where
+  head : Name.Head
+  tail : List Name.Tail
+  deriving DecidableEq, Hashable, Repr
+
+
+def Name.toList (name : Name) : List Char :=
+  name.head.val :: name.tail.map (·.val)
+
+
+def Name.toString (name : Name) : String := name.toList.asString
+instance : ToString Name where toString name := name.toString
+
+
+def Name.toFormat (name : Name) : Std.Format := name.toString.toFormat
+instance : Std.ToFormat Name where format name := name.toFormat
+
+
+def Name.of (str : List Char) : Option Name :=
+  match str with
+  | [] => none
+  | head :: tail =>
+    if h_head : isHead head then
+      if h_tail : ∀ c ∈ tail, isTail c then
+        let tail := tail.attachWith _ h_tail
+        some <| Name.mk (Subtype.mk _ h_head) tail
+      else none
+    else none
+
+
+#assert (Name.of "yogev".toList |>.isSome) == true
+
+
+instance : Inhabited Name := by
+  let x := Name.of "a".toList
+  have h : x.isSome := by decide
+  constructor
+  exact x.get h
