Interpreter/Types/Ty.lean
@@ -1,0 +1,7 @@
+namespace Interpreter.Types
+
+
+inductive Ty
+  | int
+  | bool
+  deriving Inhabited, DecidableEq, Hashable, Repr
