Interpreter/Types/Val.lean
@@ -1,0 +1,30 @@
+import Interpreter.Types.Ty
+
+
+namespace Interpreter.Types
+
+
+def Val : Ty -> Type
+  | .int => Int
+  | .bool => Bool
+
+
+variable {ty : Ty}
+
+
+--- This macro infers the underlying instance of the type `Val ty`
+syntax "underlying_instance" Lean.Parser.Tactic.elimTarget : tactic
+macro_rules
+  | `(tactic| underlying_instance $ty) =>
+    `(tactic|
+      cases $ty;
+      all_goals
+        unfold Val
+        infer_instance)
+
+
+instance : Inhabited (Val ty) := by underlying_instance ty
+instance : Repr (Val ty) := by underlying_instance ty
+instance : ToString (Val ty) := by underlying_instance ty
+instance : DecidableEq (Val ty) := by underlying_instance ty
+instance : Hashable (Val ty) := by underlying_instance ty
