Interpreter/Types/Vars.lean
@@ -1,0 +1,101 @@
+import Interpreter.Types.Ty
+import Interpreter.Types.Val
+import Interpreter.Types.Name
+import Std.Data.HashMap
+import Std.Data.HashMap.Lemmas
+import Utils.Key
+
+
+namespace Interpreter.Types
+open Std (HashMap DHashMap)
+
+
+abbrev VarTypes := HashMap Name Ty
+
+
+abbrev TyVal := (ty : Ty) × Val ty
+structure VarValues (varTypes : VarTypes) where
+  hashMap : HashMap Name TyVal
+  full : ∀ k, k ∈ hashMap <-> k ∈ varTypes
+  types_eq : ∀ k, (h : k ∈ hashMap) -> hashMap[k].fst = varTypes[k]'(full k |>.mp h)
+  deriving Repr
+
+
+-- TODO: These will be added as lemmas in 4.20. Upgrade!
+@[simp]
+axiom Std.HashMap.mem_map_iff
+{K α β : Type _} [BEq K] [Hashable K]
+{k : K} {f : K -> α -> β} {hm : HashMap K α}
+: k ∈ hm.map f <-> k ∈ hm
+@[simp]
+axiom Std.HashMap.getElem_map
+{K α β : Type _} [BEq K] [Hashable K]
+{k : K} {f : K -> α -> β} {hm : HashMap K α}
+{k_mem_hm : k ∈ hm}
+: (hm.map f)[k]'(by simp_all only [mem_map_iff]) = f k hm[k]
+
+
+variable {vt : VarTypes}
+instance : Inhabited (VarValues vt) := ⟨{
+    -- hashMap := vt.map fun name ty => ⟨ty, default⟩ -- Too hard to prove
+    hashMap := vt.map fun _ ty => ⟨ty, default⟩
+    full k := by
+      rw [Std.HashMap.mem_map_iff]
+    types_eq name name_mem_vt := by
+      rw [Std.HashMap.mem_map_iff] at name_mem_vt
+      rw [Std.HashMap.getElem_map]
+  }⟩
+instance : EmptyCollection (VarValues {}) := ⟨{
+    hashMap := {}
+    full k := by apply Iff.intro <;> simp
+    types_eq k h := by exfalso ; simp_all only [Std.HashMap.not_mem_empty]
+  }⟩
+instance : Membership Name (VarValues vt) where
+  mem vv k := k ∈ vv.hashMap
+instance : GetElem (VarValues vt) Name TyVal (fun vt name => name ∈ vt) where
+  getElem vv k k_mem_vv := vv.hashMap[k]
+
+
+-- instance {k v} [BEq k] [Hashable k]
+-- : LawfulEmptyCollectionMembership k (HashMap k v) where
+--   mem_empty _ := HashMap.not_mem_empty
+-- 
+-- 
+
+
+@[simp]
+theorem VarValues.mem_iff {name : Name} {vv : VarValues vt}
+: name ∈ vv <-> name ∈ vt :=
+  vv.full name
+@[simp]
+theorem VarValues.fst_getElem {name : Name} {vv : VarValues vt}
+{name_mem_vv : name ∈ vv}
+: vv[name].fst = vt[name]'(vv.full name |>.mp name_mem_vv) := by
+  change vv.hashMap[name].fst = _
+  exact vv.types_eq name name_mem_vv
+
+
+def VarValues.insert
+(name : Name) {ty : Ty} (val : Val ty) (vv : VarValues vt)
+: VarValues $ vt.insert name ty :=
+  {
+    hashMap := vv.hashMap.insert name ⟨ty, val⟩
+    full k := by
+      rw [HashMap.mem_insert, HashMap.mem_insert, beq_iff_eq]
+      apply Iff.intro
+      all_goals
+        rintro (name_eq_k | k_mem_vv)
+        . -- name = k
+          left
+          assumption
+        . -- k ∈ vv.hashMap
+          right
+          first | apply (vv.full k).mp | apply (vv.full k).mpr
+          assumption
+    types_eq k k_mem_vv_insert := by
+      rw [HashMap.getElem_insert, HashMap.getElem_insert]
+      by_cases h : name = k
+      . simp_all only [beq_self_eq_true, dite_true]
+      . simp_all only [beq_iff_eq, dite_false]
+        rw [vv.types_eq k]
+  }
