Utils/Key.lean
@@ -1,0 +1,69 @@
+private instance {α} {p : α -> Prop} [BEq α] : BEq (Subtype p) where
+  beq x y := x.val == y.val
+private instance {α} {p : α -> Prop} [Hashable α] : Hashable (Subtype p) where
+  hash x := hash x.val
+
+
+variable
+  {α : Type} {key : Type}
+  [membership : Membership key α]
+  {a : α} {k : key}
+
+
+@[ext]
+structure Key (a : α) where
+  val : key
+  mem : val ∈ a
+  deriving Repr
+
+
+@[simp]
+theorem Key.eq_iff {k1 k2 : Key a}
+: k1 = k2 <-> k1.val = k2.val := by
+  apply Iff.intro
+  . intro h
+    subst h
+    rfl
+  . intro h
+    ext
+    exact h
+
+
+instance [inst : DecidableEq key] : DecidableEq (Key a) := fun x y => by
+  rw [Key.eq_iff]
+  exact inst x.val y.val
+
+
+instance [Hashable key] : Hashable (Key a) where
+  hash k := hash k.val
+
+
+instance : CoeHead (Key a) key where coe k := k.val
+
+
+@[simp]
+theorem Key.mem_val (k : Key a) : k.val ∈ a := k.mem
+
+
+class LawfulEmptyCollectionMembership
+(β : Type) (α : Type)
+[EmptyCollection α]
+[Membership β α]
+where
+  mem_empty : ∀ b : β, b ∉ (∅ : α)
+attribute [simp] LawfulEmptyCollectionMembership.mem_empty
+
+
+@[simp]
+theorem Key.key_empty
+[EmptyCollection α]
+[LawfulEmptyCollectionMembership key α]
+: Key (∅ : α) -> False := by
+  intro k
+  apply absurd k.mem_val
+  exact LawfulEmptyCollectionMembership.mem_empty k.val
+
+
+@[simp]
+theorem Key.val_mk {val mem}
+: Key.val (Key.mk val mem : Key a) = (val : key) := rfl
